src/lowparse/pulse/LowParse.PulseParse.Projectors.fst
@@ -95,3 +95,77 @@ let vmatch_and
   (x': t')
 : Tot slprop
 = r1 x x' ** r2 x x'
+
+(* ========== zero_copy_parse_strong_prefix with projector ========== *)
+
+module Trade = Pulse.Lib.Trade.Util
+module S = Pulse.Lib.Slice
+module LPS = LowParse.Pulse.Base
+module PPB = LowParse.PulseParse.Base
+
+let vmatch_dep_pair_with_proj_content
+  (#t0 #t1 #t1': Type0)
+  (#t2': (t1' -> Type0))
+  (r1: t1 -> t1' -> slprop)
+  (proj: pair_proj t0 t1)
+  (r2: ((x1': t1') -> t0 -> t2' x1' -> slprop))
+  (xh: t1')
+  (x0: t0)
+  (xh2: t2' xh)
+: Tot slprop
+= r1 (proj.pair_proj_get x0) xh ** r2 xh x0 xh2
+
+#push-options "--z3rlimit 64"
+
+inline_for_extraction
+fn read_and_zero_copy_parse_strong_prefix_dtuple2_with_proj
+  (#t0 #t1 #t1': Type0)
+  (#t2': (t1' -> Type0))
+  (#k1: Ghost.erased parser_kind)
+  (#p1: parser k1 t1')
+  (#k2: Ghost.erased parser_kind)
+  (#p2: (x: t1') -> parser k2 (t2' x))
+  (r1: t1 -> t1' -> slprop)
+  (proj: pair_proj t0 t1)
+  (r2: ((x1': t1') -> t0 -> t2' x1' -> slprop))
+  (j1: LPS.jumper p1)
+  (rd1: PPB.leaf_reader p1)
+  (sq: squash (k1.parser_kind_subkind == Some ParserStrong))
+  (w2: (xh: t1') -> PPB.zero_copy_parse_strong_prefix #t0 #(t2' xh)
+    (vmatch_dep_pair_with_proj_content r1 proj r2 xh)
+    #k2 (p2 xh))
+: PPB.zero_copy_parse_strong_prefix #t0 #(dtuple2 t1' t2')
+    (vmatch_dep_pair_with_proj r1 proj r2)
+    #(and_then_kind k1 k2)
+    (parse_dtuple2 p1 p2)
+= (input: S.slice byte)
+  (#pm: perm)
+  (#v: Ghost.erased (dtuple2 t1' t2'))
+{
+  PPB.pts_to_parsed_strong_prefix_elim input;
+  with w . assert (S.pts_to input #pm w);
+  parse_dtuple2_eq p1 p2 w;
+  parser_kind_prop_equiv k1 p1;
+  let off1 = j1 input 0sz;
+  let input1, input2 = Pulse.Lib.Slice.Util.split_trade input off1;
+  with wb1 . assert (S.pts_to input1 #pm wb1);
+  with wb2 . assert (S.pts_to input2 #pm wb2);
+  Trade.trans (S.pts_to input1 #pm wb1 ** S.pts_to input2 #pm wb2) (S.pts_to input #pm w) (PPB.pts_to_parsed_strong_prefix (parse_dtuple2 p1 p2) input #pm v);
+  parse_strong_prefix p1 w wb1;
+  PPB.pts_to_parsed_intro p1 input1 (dfst v);
+  PPB.pts_to_parsed_strong_prefix_intro (p2 (dfst v)) input2 (dsnd v);
+  Trade.prod (PPB.pts_to_parsed p1 input1 #(pm /. 2.0R) (dfst v)) (S.pts_to input1 #pm wb1) (PPB.pts_to_parsed_strong_prefix (p2 (dfst v)) input2 #(pm /. 2.0R) (dsnd v)) (S.pts_to input2 #pm wb2);
+  Trade.trans (PPB.pts_to_parsed p1 input1 #(pm /. 2.0R) (dfst v) ** PPB.pts_to_parsed_strong_prefix (p2 (dfst v)) input2 #(pm /. 2.0R) (dsnd v)) (S.pts_to input1 #pm wb1 ** S.pts_to input2 #pm wb2) (PPB.pts_to_parsed_strong_prefix (parse_dtuple2 p1 p2) input #pm v);
+  let v1 = rd1 input1;
+  Trade.elim_hyp_l _ _ _;
+  rewrite each (dfst v) as v1;
+  let res = w2 v1 input2;
+  Trade.trans (vmatch_dep_pair_with_proj_content r1 proj r2 v1 res _) _ _;
+  Trade.rewrite_with_trade
+    (vmatch_dep_pair_with_proj_content r1 proj r2 v1 res _)
+    (vmatch_dep_pair_with_proj r1 proj r2 res v);
+  Trade.trans (vmatch_dep_pair_with_proj r1 proj r2 res v) _ _;
+  res
+}
+
+#pop-options
